candle/prover/candle_prover_evaluateScript.sml
@@ -603,6 +603,12 @@ Proof
     \\ first_assum (irule_at Any)
     \\ simp [Boolv_def]
     \\ rw [v_ok_def])
+  \\ Cases_on ‘∃test ty. op = Test test ty’ \\ gs []
+  >- (
+    rw [do_app_cases] \\ gs [SF SFY_ss]
+    \\ first_assum (irule_at Any)
+    \\ simp [Boolv_def]
+    \\ rw [v_ok_def])
   \\ Cases_on ‘op = Opderef’ \\ gs []
   >- (
     rw [do_app_cases] \\ gs [SF SFY_ss]
